Weidenbach_Book/IsaSAT/IsaSAT_VMTF.thy
@@ -1327,10 +1327,10 @@ definition (in -) find_decomp_wl_st :: \<open>nat literal \<Rightarrow> nat twl_
 
 definition find_decomp_wl_st_int :: \<open>nat \<Rightarrow> twl_st_wl_heur \<Rightarrow> twl_st_wl_heur nres\<close> where
   \<open>find_decomp_wl_st_int = (\<lambda>highest (M, N, D, j, W, vm, clvls, cach, lbd, outl, stats, heur,
-       vdom, avdom, lcount, opts, old_arena). do{
+       vdom, lcount, opts, old_arena). do{
      (M', vm) \<leftarrow> isa_find_decomp_wl_imp M highest vm;
      RETURN (M', N, D, j, W, vm, clvls, cach, lbd, outl, stats, heur,
-       vdom, avdom, lcount, opts, old_arena)
+       vdom, lcount, opts, old_arena)
   })\<close>
 
 lemma
